Reversal.thy
@@ -3,37 +3,163 @@ imports VCG
 begin
 
 locale list_rev_example =
-fixes i::string and j::string and k::string and it::int
+fixes i::string and j::string and k::string and \<alpha>\<^sub>0::"nat list"
+assumes a1:"i \<noteq> k" and a2:"i \<noteq> j" and a3:"j \<noteq> k"
 begin
 
 abbreviation update_mem
   where "update_mem f s \<equiv> State (f (mem s)) (vars s)"
 
 abbreviation init where
-"init \<equiv> BASIC (\<lambda>s. update_mem (\<lambda>m . m((vars s) j := 0, it := (vars s) i)) s)"
+"init \<equiv> BASIC (\<lambda>s. State (mem s) ((vars s)(j := 0)))"
 
-abbreviation list_rev where
-"list_rev \<equiv> BASIC (\<lambda>s. update_mem (\<lambda>m . m((vars s) k := (mem s) ((vars s) i + 1), (mem s) ((vars s) i + 1) := (vars s) j, (vars s) j := (vars s) i, (vars s) i := (vars s) k)) s)"
+abbreviation all where
+"all \<equiv> BASIC (\<lambda>s. State ((mem s)((mem s) ((vars s) i + 1) := (vars s) j)) ((vars s)(k := (mem s) ((vars s) i + 1), j := (vars s) i, i := (mem s)(((vars s) i) + 1))))"
 
-abbreviation pre0::"assn" where "pre0 \<equiv> \<lambda>s. \<exists>\<alpha> \<beta>. (list s \<alpha> ((vars s) i)) \<and> (list s \<beta> ((vars s) j)) \<and> (rev \<alpha> = (append (rev \<alpha>) \<beta>)) \<and> 
-  (\<forall>k::string. (reach s ((vars s) i) ((vars s) k)) \<and> (reach s ((vars s) j) ((vars s) k)) \<longrightarrow> ((vars s) k = 0))"
+abbreviation assgin1 where
+"assgin1 \<equiv> BASIC (\<lambda>s. State (mem s) ((vars s)(k := (mem s) ((vars s) i + 1))))"
 
-abbreviation inv::"assn" where "inv \<equiv> \<lambda>s. \<exists>\<alpha> \<beta> \<alpha>\<^sub>0. (list s \<alpha> ((vars s) i)) \<and> (list s \<beta> ((vars s) j))  \<and> (list s \<alpha>\<^sub>0 it) \<and> (rev \<alpha>\<^sub>0 = (append (rev \<alpha>) \<beta>)) \<and> 
-  (\<forall>k::string. (reach s ((vars s) i) ((vars s) k)) \<and> (reach s ((vars s) j) ((vars s) k)) \<longrightarrow> ((vars s) k = 0))"
+abbreviation assgin2 where
+"assgin2 \<equiv> BASIC (\<lambda>s. State ((mem s)((mem s) ((vars s) i + 1) := (vars s) j)) (vars s))"
 
-abbreviation post::"assn" where "post \<equiv> \<lambda>s. \<exists>\<alpha> \<beta> \<alpha>\<^sub>0. (list s \<alpha> ((vars s) i)) \<and> (list s \<beta> ((vars s) j)) \<and> (list s \<alpha>\<^sub>0 it) \<and> (rev \<alpha>\<^sub>0 = (append (rev \<alpha>) \<beta>)) \<and> 
-  (\<forall>k::string. (reach s ((vars s) i) ((vars s) k)) \<and> (reach s ((vars s) j) ((vars s) k)) \<longrightarrow> ((vars s) k = 0))"
+abbreviation assign3 where
+"assign3 \<equiv> BASIC (\<lambda>s. State (mem s) ((vars s)(j := (vars s) i)))"
+
+abbreviation assign4 where
+"assign4 \<equiv> BASIC (\<lambda>s. State (mem s) ((vars s)(i := (vars s) k)))"
+
+abbreviation pre0::"assn" where "pre0 \<equiv> \<lambda>s. \<exists>\<alpha> \<beta>. ((vars s) i \<noteq> 0) \<and> ((vars s) j = 0) \<and> (list s  \<alpha>\<^sub>0 ((vars s) i)) \<and>  (list s \<alpha> ((vars s) i)) \<and> 
+  (list s \<beta> ((vars s) j)) \<and> (rev \<alpha>\<^sub>0 = (append (rev \<alpha>) \<beta>)) \<and> (\<forall>k::string. (reach s ((vars s) i) ((vars s) k)) \<and> (reach s ((vars s) j) ((vars s) k)) \<longrightarrow> ((vars s) k = 0))"
+
+definition inv::"assn" where "inv \<equiv> \<lambda>s. \<exists>\<alpha> \<beta>. (list s \<alpha> ((vars s) i)) \<and> (list s \<beta> ((vars s) j)) \<and> (rev \<alpha>\<^sub>0 = (append (rev \<alpha>) \<beta>))
+  \<and> (\<forall> v . (reach s ((vars s) i) v) \<and> (reach s ((vars s) j) v) \<longrightarrow> v = 0)"
+
+abbreviation post::"assn" where "post \<equiv> \<lambda>s. \<exists>\<alpha> \<beta>. (list s \<alpha> 0) \<and> (list s \<beta> ((vars s) j)) \<and> (rev \<alpha>\<^sub>0 = (append (rev \<alpha>) \<beta>)) \<and> 
+  (\<forall>k::string. (reach s 0 ((vars s) k)) \<and> (reach s ((vars s) j) ((vars s) k)) \<longrightarrow> ((vars s) k = 0))"
 
 abbreviation loopcom::com where 
-"loopcom \<equiv> init;; WHILE (\<lambda>s. (vars s) i \<noteq> 0) INV inv DO list_rev OD"
+"loopcom \<equiv> init;; WHILE (\<lambda>s. (vars s) i \<noteq> 0) INV inv DO ((assgin1;; assgin2);; assign3);; assign4 OD"
 
+lemma l2:
+  fixes s s' l v
+  assumes "mem s = mem s'"
+  shows "list s l v = list s' l v" using assms
+by (induct rule: list.induct) simp_all
+
+lemma l3:
+  fixes s s'
+  assumes "list s l ((vars s) v)" and "mem s = mem s'" and "(vars s) v = ((vars s') v)"
+  shows "list s' l ((vars s') v)" using assms
+by (metis l2) 
+
+lemma l4:
+  fixes s s' l v
+  assumes "mem s = mem s'"
+  shows "reach_step s n addr v = reach_step s' n addr v" using assms
+apply (induct rule:reach_step.induct) apply auto done
+
+lemma l5:
+  fixes s s' l v
+  assumes "mem s = mem s'"
+  shows "reach s addr v = reach s' addr v" using assms
+by (metis l4 reach_def)
+
+lemma l6:
+  fixes s v
+  assumes "local.inv s"
+  shows "local.inv (State (mem s) ((vars s)(k := v)))"
+using assms
+by (smt a1 a3 fun_upd_apply l2 l5 local.inv_def newstate.sel(1) newstate.sel(2)) 
+
+lemma l7:
+  assumes "list s \<alpha> a1" and "(mem s) a2 = v" and "(mem s) (a2 + 1) = a1"
+  shows "list s (v#\<alpha>) a2" using assms
+by (induct \<alpha>) simp_all
+
+thm list.induct
+
+lemma l8:
+  assumes "list s \<alpha> addr" and "\<alpha> \<noteq> []"
+  shows "(mem s) (addr + 1) \<noteq> addr" using assms
+  proof (induct \<alpha>)
+    print_cases
+    case (Cons x xs) thus ?case 
+    apply (induct xs) 
+  
+
+lemma "\<turnstile>\<^sub>t\<^sub>r {\<lambda> s . \<alpha> \<noteq> [] \<and> ((vars s) i \<noteq> 0) \<and> inv s \<and> list s \<alpha> ((vars s) i) \<and> list s \<beta> ((vars s) j)} BASIC (\<lambda> s . State (mem s) ((vars s)(k := ((mem s) (((vars s) i) + 1))))) 
+  {\<lambda> s . \<alpha> \<noteq> [] \<and> ((vars s) i \<noteq> 0) \<and> inv s \<and> list s (tl \<alpha>) ((vars s) k) \<and> list s \<alpha> ((vars s) i) \<and> list s \<beta> ((vars s) j) \<and> ((vars s) k) \<noteq> ((vars s) i) + 1}" 
+apply (rule Basic)
+by (smt Ann_Com.list.simps(2) a1 a3 fun_upd_apply l2 l6 list.collapse newstate.sel(1) newstate.sel(2)) 
+
+lemma "\<turnstile>\<^sub>t\<^sub>r {\<lambda> s . \<alpha> \<noteq> [] \<and> ((vars s) i \<noteq> 0) \<and> inv s \<and> list s (tl \<alpha>) ((vars s) k) \<and> list s \<alpha> ((vars s) i) \<and> list s \<beta> ((vars s) j)} 
+  BASIC (\<lambda>s. State ((mem s)(((vars s) i + 1) := (vars s) j)) (vars s)) 
+  {\<lambda> s . \<alpha> \<noteq> [] \<and> ((vars s) i \<noteq> 0) \<and> list s (tl \<alpha>) ((vars s) k)}"
+apply (rule Basic) nitpick[show_consts]
+
+lemma "\<turnstile>\<^sub>t\<^sub>r {\<lambda> s . \<alpha> \<noteq> [] \<and> ((vars s) i \<noteq> 0) \<and> inv s \<and> list s (tl \<alpha>) ((vars s) k) \<and> list s \<alpha> ((vars s) i) \<and> list s \<beta> ((vars s) j)} 
+  BASIC (\<lambda>s. State ((mem s)((mem s) ((vars s) i + 1) := (vars s) j)) (vars s)) 
+  {\<lambda> s . \<alpha> \<noteq> [] \<and> ((vars s) i \<noteq> 0) \<and> list s (tl \<alpha>) ((vars s) k) \<and> list s \<beta> ((vars s) j) \<and> list s ((hd \<alpha>)#\<beta>) ((vars s) i)}"
+apply (rule Basic) 
+
+lemma "inv s \<Longrightarrow> pre_tr all local.inv s" 
+
+
+(*
 lemma "\<turnstile>\<^sub>t\<^sub>r {pre0} loopcom {post}"
-apply(rule Seq)
+apply(rule Seq[where Q=inv])
+apply(rule Basic)
+apply (metis fun_upd_triv newstate.collapse)
+apply(rule While)
+apply simp
+prefer 2
+apply force
+apply(insert vc_sound_tr[where Q="inv" and c="((assgin1;; assgin2);; assign3);; assign4"])
+apply(rule conseq[where P="pre_tr ((assgin1;; assgin2);; assign3);; assign4 local.inv" and P'="\<lambda>s. local.inv s \<and> vars s i \<noteq> 0" and Q="inv" and Q'="inv"])
+prefer 3
+
+
+
+
 prefer 2
 apply(rule While [where P = inv])
 apply simp
-sorry
+prefer 2
+apply force
+prefer 2
+apply(rule Basic)
+apply simp
+apply(smt fun_upd_triv newstate.collapse)
+apply (rule Seq [where Q = "\<lambda>s. local.inv s \<and> vars s i \<noteq> 0"])
+prefer 2
+apply(rule Basic)
+apply simp
+proof
+  fix s
+  have "(j = i \<longrightarrow>
+         (\<exists>\<alpha>. list s \<alpha> (vars s i) \<and> (\<exists>\<beta>. list s \<beta> (vars s i) \<and> rev \<alpha>\<^sub>0 = rev \<alpha> @ \<beta> \<and> (\<forall>k. reach s (vars s i) (vars s k) \<longrightarrow> vars s k = 0))) \<and> vars s i \<noteq> 0 \<longrightarrow>
+         (\<exists>\<alpha>. list (State (mem s) ((vars s)(i := vars s k))) \<alpha> (vars s k) \<and>
+               (\<exists>\<beta>. list (State (mem s) ((vars s)(i := vars s k))) \<beta> (vars s k) \<and>
+                    rev \<alpha>\<^sub>0 = rev \<alpha> @ \<beta> \<and>
+                    (\<forall>ka. (ka = i \<longrightarrow> reach (State (mem s) ((vars s)(i := vars s k))) (vars s k) (vars s k) \<longrightarrow> vars s k = 0) \<and>
+                          (ka \<noteq> i \<longrightarrow> reach (State (mem s) ((vars s)(i := vars s k))) (vars s k) (vars s ka) \<longrightarrow> vars s ka = 0)))))"
+using reach_def reach_step.simps(1) by blast
+  have " j \<noteq> i \<longrightarrow>
+          (\<exists>\<alpha>. list s \<alpha> (vars s i) \<and> (\<exists>\<beta>. list s \<beta> (vars s j) \<and> rev \<alpha>\<^sub>0 = rev \<alpha> @ \<beta> \<and> (\<forall>k. reach s (vars s i) (vars s k) \<and> reach s (vars s j) (vars s k) \<longrightarrow> vars s k = 0))) \<and>
+          vars s i \<noteq> 0 \<longrightarrow>
+          (\<exists>\<alpha>. list (State (mem s) ((vars s)(i := vars s k))) \<alpha> (vars s k) \<and>
+                (\<exists>\<beta>. list (State (mem s) ((vars s)(i := vars s k))) \<beta> (vars s j) \<and>
+                     rev \<alpha>\<^sub>0 = rev \<alpha> @ \<beta> \<and>
+                     (\<forall>ka. (ka = i \<longrightarrow>
+                            reach (State (mem s) ((vars s)(i := vars s k))) (vars s k) (vars s k) \<and> reach (State (mem s) ((vars s)(i := vars s k))) (vars s j) (vars s k) \<longrightarrow>
+                            vars s k = 0) \<and>
+                           (ka \<noteq> i \<longrightarrow>
+                            reach (State (mem s) ((vars s)(i := vars s k))) (vars s k) (vars s ka) \<and> reach (State (mem s) ((vars s)(i := vars s k))) (vars s j) (vars s ka) \<longrightarrow>
+                            vars s ka = 0))))"
+  proof
 
+sorry
+*)
 end
 
 end
